

IV.3. Let  $x$  be any positive real number. Then show that for all natural numbers  $n$ , the following inequality holds:

$$(1 + x)^n \geq 1 + nx$$

*Hint: Use induction on  $n$*

**Base Case:** ( $n=1$ )

$$(1 + x)^1 \geq 1 + 1x$$

$$1 + x = 1 + x$$

**Induction hypothesis:**

Assume for some arbitrary positive integers  $k \geq 1$

that:

$$(1 + x)^k \geq 1 + kx \quad \text{where } x > 0$$

We assume that statement is true for  $n = k$  to prove it for  $n = k + 1$

We need to show:

$$(1 + x)^{k+1} \geq 1 + (k + 1)x$$

$$\text{LHS} = (1 + x)^{k+1} = (1 + x)^k(1 + x)$$

$x$  is a positive real number, so we can multiply both side of the Inductive hypothesis by  $(1 + x)$

And doing so will not change the direction of the inequality:

$$(1 + x)^k(1 + x) \geq (1 + kx)(1 + x)$$

$$(1 + x)^k(1 + x) \geq 1 + x + kx + kx^2$$

$$(1 + x)^k(1 + x) \geq 1 + (k + 1)x + kx^2$$

$k$  being a positive integer and  $x$  being a positive real number making  $kx^2$  a strictly positive ( $kx^2 > 0$ )

By knowing ( $kx^2 > 0$ ), we can state that:

$$1 + (k + 1)x + kx^2 \geq 1 + (k + 1)x$$

**Combining the steps:**

$$(1 + x)^{k+1} \geq (1 + kx)(1 + x) = 1 + (k + 1)x + kx^2 \geq 1 + (k + 1)x$$

Thus, we have successfully show that the statement  $((1 + x)^{k+1} \geq 1 + (k + 1)x)$  is true. ■